Assignment/Semantics_Inline_func.v
@@ -1,0 +1,164 @@
+Require Import Coq.Logic.Classical_Prop.
+Require Import Coq.Strings.String.
+Require Import Coq.ZArith.ZArith.
+Require Import Coq.micromega.Psatz.
+Require Import Coq.Classes.Equivalence.
+Require Import Coq.Classes.Morphisms.
+Require Import SetsClass.SetsClass. Import SetsNotation.
+Require Import PL.InductiveType.
+Require Import PL.RecurProp.
+Require Import PL.Monad2.
+Require Import Assignment.Syntax.
+Require Import Assignment.FuncEquiv.
+Require Import Coq.Lists.List.
+Require Import Assignment.Semantics.
+Local Open Scope string.
+Local Open Scope Z.
+Local Open Scope sets.
+
+Module Semantics_SimpleWhileFunc_Inline.
+Import StateRelMonad.
+Import Lang_SimpleWhileFunc.
+Import Semantics_SimpleWhileFunc.
+
+Fixpoint get_args (args: list Z) (i: Z): Z := 
+  match args with
+  | nil => 0
+  | cons arg args' => 
+    match i with
+    | Z0 => arg
+    | _ => get_args args' (i-1)
+    end
+  end.
+
+Definition args_sem (args: list Z) (i: Z): expr_int_sem :=
+  fun (s1: state) (res: Z) (s2: state) => 
+  res = get_args args i /\ s1 = s2.
+
+Fixpoint eval_expr_func (e: expr_func) (args: list Z) : expr_int_sem := 
+  match e with
+  | EFConst n => const_sem n
+  | EFVar X => var_sem X
+  | EFArgs i => args_sem args i
+  | EFAdd e1 e2 => add_sem (eval_expr_func e1 args) (eval_expr_func e2 args)
+  | EFSub e1 e2 => sub_sem (eval_expr_func e1 args) (eval_expr_func e2 args)
+  | EFMul e1 e2 => mul_sem (eval_expr_func e1 args) (eval_expr_func e2 args)
+  end.
+
+#[export] Instance args_sem_congr:
+  Proper (eq ==> eq ==> Sets.equiv) args_sem.
+Proof.
+  unfold Proper, respectful.
+  intros.
+  unfold args_sem.
+  rewrite H. rewrite H0.
+  reflexivity.
+Qed.
+
+Fixpoint get_args_inline (args: list expr_int) (i: Z): expr_int := 
+  match args with
+  | nil => EConst 0
+  | cons arg args' => 
+    match i with
+    | Z0 => arg
+    | _ => get_args_inline args' (i-1)
+    end
+  end.
+
+Fixpoint translate_func_inline (e: expr_func) (args: list expr_int) : expr_int :=
+  match e with
+  | EFConst n => EConst n
+  | EFVar X => EVar X
+  | EFArgs i => get_args_inline args i
+  | EFAdd e1 e2 => EAdd (translate_func_inline e1 args) (translate_func_inline e2 args)
+  | EFSub e1 e2 => ESub (translate_func_inline e1 args) (translate_func_inline e2 args)
+  | EFMul e1 e2 => EMul (translate_func_inline e1 args) (translate_func_inline e2 args)
+  end.
+
+Definition state_unchanged (fs: func_list) (e: expr_int): Prop :=
+  forall s1 res s2, (s1, res, s2) ∈ (eval_expr_int fs e) -> s1 = s2.
+
+Fixpoint list_state_unchanged (fs: func_list) (args: list expr_int): Prop :=
+  match args with
+  | nil => True
+  | cons e args' => state_unchanged fs e /\ list_state_unchanged fs args'
+  end.
+
+Lemma bind_args_unchanged:
+  forall fs args, (list_state_unchanged fs args -> 
+    (forall s1 Dargs s2, 
+      ((s1, Dargs, s2) ∈ bind_args (map (eval_expr_int fs) args) ->
+        s1 = s2))).
+Proof.
+  intros.
+  revert H0. revert s1 Dargs s2.
+  induction args.
+  + intros. unfold map, bind_args, ret in H0.
+    sets_unfold in H0. tauto.
+  + intros.
+    unfold list_state_unchanged in H. destruct H as [? ?].
+    fold list_state_unchanged in H1. specialize (IHargs H1).
+    sets_unfold in H0. unfold bind_args, map in H0.
+    fold bind_args in H0.
+    change (((fix map (l : list expr_int) :
+          list expr_int_sem :=
+        match l with
+        | nil => nil
+        | a :: t => eval_expr_int fs a :: map t
+        end) args)) with (map (eval_expr_int fs) args) in H0.
+    unfold append_arg in H0. destruct H0 as [s3 ?]. 
+    destruct H0 as [Dargs0 ?]. destruct H0 as [arg ?].
+    destruct H0 as (H2 & H3 & H4). 
+    specialize (IHargs s3 Dargs0 s2 H3).
+    apply H in H4.
+    rewrite H4, <- IHargs.
+    reflexivity.
+Qed.
+
+Lemma inline_const_sem:
+  forall fs n args, 
+    list_state_unchanged fs args ->
+    Sets.equiv
+      (func_sem (eval_expr_func (EFConst n))
+      (map (eval_expr_int fs) args))
+      (const_sem n).
+Proof.
+  intros.
+  unfold eval_expr_func.
+  unfold func_sem.
+  split; revert a a0 a1.
+  + intros s1 res s2. intros. destruct H0 as [s3 H0]. destruct H0 as [args0 H0]. destruct H0 as [res1 H0].
+    destruct H0 as [? ?].
+    pose proof (bind_args_unchanged fs args H).
+    apply H2 in H0. rewrite H0.
+    sets_unfold in H1.
+    unfold const_sem. unfold const_sem in H1.
+
+
+
+Lemma inline_equivalence:
+  forall fs f e args, 
+    eq (fs f) (eval_expr_func e) ->
+    Sets.equiv
+    (eval_expr_int fs (translate_func_inline e args)) 
+    (eval_expr_int fs (EFunc f args)).
+Proof.
+  intros.
+  unfold eval_expr_int.
+  fold eval_expr_int.
+  rewrite H.
+  induction e.
+  + unfold translate_func_inline. eval_expr_func.
+    change ((fun _ : list Z => const_sem n)
+            (map (eval_expr_int fs) args))
+            with (const_sem n).
+  split.
+  unfold translate_func_inline.
+
+
+
+
+
+
+
+End Semantics_SimpleWhileFunc_Inline.
